src/lib/poly/gemm/Kuiper.Poly.GEMM.TensorCore2D.fsti
@@ -3,7 +3,15 @@ module Kuiper.Poly.GEMM.TensorCore2D
 #lang-pulse
 
 open Kuiper
-open Kuiper.Poly.GEMMGPU.Type
+open Kuiper.Matrix
+open Kuiper.EMatrix
+
+open Kuiper.Matrix.Reprs
+open Kuiper.TensorCore
+
+module SZ = FStar.SizeT
 
 inline_for_extraction noextract
-val mmcomb_gpu : block_tiled2d_matmulcomb_gpu_ty
+let warp_sz = 32sz
+inline_for_extraction noextract
+let warp_size = SZ.v warp_sz
